Semantics/Set.lean
@@ -2,39 +2,31 @@
 
 def Set (α: Type) := α → Prop
 
-def setOf (p: α → Prop): Set α :=
-  p
+def setOf (p: α → Prop): Set α := p
 
 namespace Set
 
-protected def Mem (s: Set α) (a: α): Prop :=
-  s a
+protected def Mem (s: Set α) (a: α): Prop := s a
 
-instance: Membership α (Set α) :=
-  ⟨Set.Mem⟩
+instance: Membership α (Set α) := ⟨Set.Mem⟩
 
-theorem ext {a b: Set α} (h: ∀ (x: α), x ∈ a ↔ x ∈ b):
-  a = b :=
-  funext (λ x ↦ propext (h x))
+theorem ext {a b: Set α} (h: ∀ (x: α), x ∈ a ↔ x ∈ b): a = b :=
+  funext (propext $ h ·)
 
 protected def Subset (s₁ s₂: Set α) :=
   ∀⦃a⦄, a ∈ s₁ → a ∈ s₂
 
-instance: LE (Set α) :=
-  ⟨Set.Subset⟩
+instance: LE (Set α) := ⟨Set.Subset⟩
 
-instance: HasSubset (Set α) :=
-  ⟨(· ≤ ·)⟩
+instance: HasSubset (Set α) := ⟨(· ≤ ·)⟩
 
-instance: EmptyCollection (Set α) :=
-  ⟨λ _ ↦ False⟩
+instance: EmptyCollection (Set α) := ⟨λ _ ↦ False⟩
 
-notation (priority := high) "{" x " | " p "}" => setOf (λ x ↦ p)
+notation (priority := high) "{" x " | " p "}" => setOf $ λ x ↦ p
 
-def univ: Set α := {_a | True}
+def univ: Set α := {_ | True}
 
-protected def insert (a: α) (s: Set α): Set α :=
-  {b | b = a ∨ b ∈ s}
+protected def insert (a: α) (s: Set α): Set α := {b | b = a ∨ b ∈ s}
 
 instance: Insert α (Set α) := ⟨Set.insert⟩
 
@@ -62,44 +54,34 @@ end Set
   ## Set theorems
 -/
 
-theorem Set.mem_comprehend
-  (a: α) (P: α → Prop):
-  a ∈ ({a | P a}: Set α) ↔ P a :=
+theorem Set.mem_comprehend (a: α) (P: α → Prop): a ∈ ({a | P a}: Set α) ↔ P a :=
   Iff.rfl
 
-theorem Set.mem_diff {s t: Set α}
-  (x: α): x ∈ s \ t ↔ x ∈ s ∧ x ∉ t :=
+theorem Set.mem_diff {s t: Set α} (x: α): x ∈ s \ t ↔ x ∈ s ∧ x ∉ t :=
   Iff.rfl
 
 /-
   ### Basic subset properties
 -/
 
-theorem Subset.refl
-  (x: Set α): x ⊆ x :=
-  λ _ ↦ id
+theorem Subset.refl (x: Set α): x ⊆ x := λ _ ↦ id
 
-theorem Subset.trans {x y z: Set α}
-  (h₁: x ⊆ y) (h₂: y ⊆ z): x ⊆ z :=
-  λ _ h ↦ h₂ (h₁ h)
+theorem Subset.trans {x y z: Set α} (hsub₁: x ⊆ y) (hsub₂: y ⊆ z): x ⊆ z :=
+  λ _ h ↦ hsub₂ $ hsub₁ h
 
-theorem Subset.antisymm {x y: Set α}
-  (hsub₁: x ⊆ y) (hsub₂: y ⊆ x): x = y :=
+theorem Subset.antisymm {x y: Set α} (hsub₁: x ⊆ y) (hsub₂: y ⊆ x): x = y :=
   funext λ _ ↦ propext ⟨(hsub₁ ·), (hsub₂ ·)⟩
 
-theorem Subset.from_eq {x y: Set α}
-  (heq: x = y): x ⊆ y :=
-  λ _ h₁ ↦ heq ▸ h₁
+theorem Subset.from_eq {x y: Set α} (heq: x = y): x ⊆ y :=
+  λ _ h ↦ heq ▸ h
 
 /-
   ### Set if then else
 -/
 
-def Set.ite (t s s': Set α): Set α :=
-  s ∩ t ∪ s' \ t
+def Set.ite (t s s': Set α): Set α := s ∩ t ∪ s' \ t
 
-theorem Set.ite_mono (t: Set α) {s₁ s₁' s₂ s₂': Set α}
-  (h: s₁ ⊆ s₂) (h': s₁' ⊆ s₂'):
+theorem Set.ite_mono (t: Set α) (h: s₁ ⊆ s₂) (h': s₁' ⊆ s₂'):
   t.ite s₁ s₁' ⊆ t.ite s₂ s₂' := λ _ h2 ↦
   match h2 with
   | Or.inl ⟨hl, hr⟩ => Or.inl ⟨h hl, hr⟩
@@ -125,28 +107,24 @@ def comp (f g: α →ˢ α): α →ˢ α :=
 
 infixl:90 " ○ " => SFun.comp
 
-theorem mem_comp {f g: α →ˢ α}:
-  x ∈ f ○ g ↔ ∃z, (x.1, z) ∈ f ∧ (z, x.2) ∈ g :=
+theorem mem_comp: x ∈ f ○ g ↔ ∃z, (x.1, z) ∈ f ∧ (z, x.2) ∈ g :=
   Iff.rfl
 
-theorem comp_mono {α: Type} {f g h k: Set (α × α)}
-  (hfh: f ⊆ h) (hgk: g ⊆ k): f ○ g ⊆ h ○ k :=
+theorem comp_mono (hfh: f ⊆ h) (hgk: g ⊆ k): f ○ g ⊆ h ○ k :=
   λ _ ⟨z, h₁, h₂⟩ ↦ ⟨z, hfh h₁, hgk h₂⟩
 
-theorem comp_id {f: α →ˢ α}: f ○ id = f := by
-  funext (_s₁, s₂)
-  apply eq_iff_iff.mpr
-  unfold comp
+theorem comp_id: f ○ id = f := by
+  apply funext
+  intro (_s₁, s₂)
+  apply propext
   constructor
   . intro ⟨z, h₁, h₂⟩
     apply mem_id.mp h₂ ▸ h₁
-  . intro h
-    exact ⟨s₂, h, rfl⟩
+  . exact (⟨s₂, ·, rfl⟩)
 
-theorem id_comp {f: α →ˢ α}: id ○ f = f := by
+theorem id_comp: id ○ f = f := by
   funext (s₁, _s₂)
-  apply eq_iff_iff.mpr
-  unfold comp
+  apply propext
   constructor
   . intro ⟨z, h₁, h₂⟩
     apply mem_id.mp h₁ ▸ h₂
